pipe is working.. but the rest is admitted

VST-introduction/ASI_kalloc.v
@@ -1,4 +1,5 @@
 Require Import VST.floyd.proofauto.
+Require Import VC.helper.
 (*Require Export malloc_lemmas.*) (*Exports the model (constants like WA , plus lemmas)*)
 
 (*Require Import malloc. needed for function and type names but not for compspecs 
@@ -20,7 +21,7 @@ Record KallocFreeAPD := {
   mem_mgr: globals -> mpred;
 }.
 
-Definition kalloc_token {cs:compspecs} K (sh: share) (t: type) (p: val): mpred := 
+(*Definition kalloc_token {cs:compspecs} K (sh: share) (t: type) (p: val): mpred := 
    !! field_compatible t [] p && 
    kalloc_token' K sh (sizeof t) p.
 
@@ -30,7 +31,7 @@ Proof. intros. unfold kalloc_token.
  apply andp_left2. apply kalloc_token'_valid_pointer.
 Qed.
 
-#[export] Hint Resolve kalloc_token'_valid_pointer : valid_pointer.
+*)#[export] Hint Resolve kalloc_token'_valid_pointer : valid_pointer. (*
 #[export] Hint Resolve kalloc_token_valid_pointer : valid_pointer.
 
 Lemma kalloc_token_local_facts:  forall {cs: compspecs} K sh t p,
@@ -40,43 +41,57 @@ Proof. intros.
  normalize. rewrite prop_and.
  apply andp_right. apply prop_right; auto.
  apply kalloc_token'_local_facts.
-Qed.
+Qed.*)
 
 #[export] Hint Resolve kalloc_token'_local_facts : saturate_local.
-#[export] Hint Resolve kalloc_token_local_facts : saturate_local.
+(*#[export] Hint Resolve kalloc_token_local_facts : saturate_local.*)
 
 Section Kalloc_ASI.
 Variable K: KallocFreeAPD.
 Variable kalloc1ID: ident.
 Variable kfree1ID: ident.
 
-Definition kalloc1_spec := 
-   DECLARE (*_kalloc*)kalloc1ID
-   WITH n:Z, gv:globals, original_freelist_pointer:val
-   PRE [ ]
-       PROP (0 <= n <= Ptrofs.max_unsigned(* - (WA+WORD)*) /\ is_pointer_or_null original_freelist_pointer)
-       PARAMS () GLOBALS (gv)
-       SEP ( mem_mgr K gv )
-   POST [ tptr tvoid ]
-       PROP ()
-       RETURN (original_freelist_pointer)
-       SEP ( mem_mgr K gv;
-             if eq_dec original_freelist_pointer nullval then emp
-             else (kalloc_token' K sh n original_freelist_pointer * memory_block sh n original_freelist_pointer)).
 
-Definition kfree1_spec :=
- DECLARE (*_kfree*)kfree1ID
-   WITH n:Z, p:val, gv: globals
-   PRE [ tptr tvoid ]
-       PROP ()
-       PARAMS (p) GLOBALS (gv)
-       SEP (mem_mgr K gv;
-            if eq_dec p nullval then emp
-            else (kalloc_token' K sh n p * memory_block sh n p))
-    POST [ Tvoid ]
-       PROP ()
-       LOCAL ()
-       SEP (mem_mgr K gv).
+Definition kfree1_spec := 
+  DECLARE kfree1ID
+      WITH t:type, new_head:val, gv:globals (*sh : share, new_head:val, original_freelist_pointer:val, xx:Z, gv:globals, ls : list val, size:Z, n:Z (* n = PGSIZE.. *)*)
+      PRE [ tptr tvoid]
+        PROP(
+              is_pointer_or_null new_head
+              ) 
+        PARAMS (new_head) GLOBALS(gv)
+        SEP (
+          mem_mgr K gv;
+          if eq_dec new_head nullval then emp
+          else (kalloc_token' K Ews (sizeof t) new_head * data_at_ Ews t new_head)
+        )
+      POST [ tvoid ]
+        PROP()
+        RETURN () 
+        SEP (
+          mem_mgr K gv
+            ).
+
+
+Definition kalloc1_spec :=
+DECLARE kalloc1ID
+WITH t:type, gv:globals (*sh : share, original_freelist_pointer:val, xx:Z, ls:list val, gv:globals, n:Z*) (* n = PGSIZE.. *)
+PRE [ ]
+    PROP(0 <= sizeof t <= PGSIZE;
+    complete_legal_cosu_type t = true;
+    natural_aligned natural_alignment t = true) 
+    PARAMS () GLOBALS(gv)
+    SEP ( mem_mgr K gv )  
+POST [ tptr tvoid ]
+  EX p:val,
+    PROP()
+    RETURN (p) (* we return the head like in the pop function*)
+    SEP (
+      mem_mgr K gv;
+      if eq_dec p nullval then emp
+      else (kalloc_token' K Ews (sizeof t) p * data_at_ Ews t p) (** TODO: fix EWs...*)
+        ).
 
 Definition Kalloc_ASI:funspecs := [kalloc1_spec; kfree1_spec].
 End Kalloc_ASI.
+        
