VST-introduction/VSU_kalloc_kfree_definitions.v
@@ -8,12 +8,18 @@ Require Import malloc_sep.*)
 (* THIS SHOULD CONTAIN ANY INTERNAL FUNCTIONS... I DON'T HAVE ANY *)
 
 
+(** token -- could be moved to another file *)
+
 Definition my_kalloc_token (sh: share) (sz: Z) (p: val) : mpred := (* my kalloc token is a block where we can have t_run struct in it, but also something else?*)
-  !! (field_compatible t_run [] p 
-      /\ malloc_compatible (sz) p
-      /\ 0 <= sizeof t_run <= sz
-      /\ writable_share sh) 
- &&  memory_block sh (sz) (p). (* this is the rest of the page*)
+  EX v,
+    !! (
+        field_compatible t_run [] p 
+        /\ malloc_compatible (sz) p
+        /\ 0 <= sizeof t_run <= sz
+        /\ writable_share sh) 
+  && ((memory_block sh (sz) (p)) * data_at sh t_run v p). (* this is the rest of the page*)
+
+  
 
 (** **** Exercise: 2 stars, standard (malloc_token_properties) *)
 Lemma my_kalloc_token_valid_pointer:
@@ -22,9 +28,9 @@ Lemma my_kalloc_token_valid_pointer:
 Proof.
   intros. 
     induction sz.
-  - unfold my_kalloc_token. simpl. entailer!.
-  - unfold my_kalloc_token. simpl. entailer!.
-  - unfold my_kalloc_token. entailer!. 
+  - unfold my_kalloc_token. simpl. entailer!. entailer.
+  - unfold my_kalloc_token. simpl. entailer!. entailer.
+  - unfold my_kalloc_token. entailer!. entailer. 
 Qed.
 
 Lemma  my_kalloc_token_local_facts : 
@@ -32,16 +38,69 @@ Lemma  my_kalloc_token_local_facts :
      my_kalloc_token sh sz p |-- !! malloc_compatible sz p.
 Proof.
   intros. 
-  unfold my_kalloc_token. simpl. entailer!.
+  unfold my_kalloc_token. simpl. entailer.
 Qed.
+
+(** token -- could be moved to another file *)
+
 
 Definition Tok_APD := Build_KallocTokenAPD my_kalloc_token my_kalloc_token_valid_pointer
    my_kalloc_token_local_facts.
 
-Definition mem_mgr (gv: globals) : mpred :=
-   EX sh: share, EX i: Z, EX p: val, EX ls: list val, EX xx, EX original_freelist_pointer,
+Definition mem_mgr (gv: globals) : mpred := (* I am unsure how to access all these elements.. *)
+EX sh: share, EX ls: list val, EX xx, EX original_freelist_pointer,
+    !! (writable_share sh /\
+        is_pointer_or_null original_freelist_pointer /\
+              (((ls = nil) /\ original_freelist_pointer = nullval) \/ 
+              ((ls <> nil) /\ isptr original_freelist_pointer))
+        ) &&
       data_at sh t_struct_kmem (Vint (Int.repr xx), original_freelist_pointer) (gv _kmem) *
       freelistrep sh ls original_freelist_pointer.
+
+(************ mem_mgr lemmas etc. *************)
+Lemma mem_mgr_split: 
+ forall gv:globals,
+  mem_mgr gv
+  = 
+  EX sh: share, EX ls: list val, EX xx, EX original_freelist_pointer,
+      !! (writable_share sh /\
+          is_pointer_or_null original_freelist_pointer /\
+          (((ls = nil) /\ original_freelist_pointer = nullval) \/ ((ls <> nil) /\ isptr original_freelist_pointer))) &&
+        data_at sh t_struct_kmem (Vint (Int.repr xx), original_freelist_pointer) (gv _kmem) *
+        freelistrep sh ls original_freelist_pointer.
+Proof.
+  intros. apply pred_ext.
+  - unfold mem_mgr. Intros sh ls xx original_freelist_pointer. entailer!.
+  Exists sh ls xx original_freelist_pointer. entailer!.
+  - Intros sh ls xx original_freelist_pointer.
+  unfold mem_mgr. Exists sh ls xx original_freelist_pointer. entailer!.
+Qed.
+
+
+Lemma kalloc_token'_split: 
+ forall  (sh: share) (sz: Z) (p: val),
+ my_kalloc_token  (sh) (sz) (p)
+  = 
+  EX v,
+    !! (
+        field_compatible t_run [] p 
+        /\ malloc_compatible (sz) p
+        /\ 0 <= sizeof t_run <= sz
+        /\ writable_share sh) 
+  && ((memory_block sh (sz) (p)) * data_at sh t_run v p). 
+Proof.
+  intros. apply pred_ext.
+  - unfold my_kalloc_token. entailer!. Exists v. entailer!.
+  - unfold my_kalloc_token. entailer!. Exists v. entailer!.
+Qed.
+
+
+
+(************ mem_mgr lemmas etc. end *************)
+
+
+
+
 
 Definition KF_APD := Build_KallocFreeAPD Tok_APD mem_mgr.
 
@@ -60,3 +119,4 @@ Definition MF_Gprog:funspecs := (*MF_Imports ++*) MF_internal_specs.
 (* I don't think I have any internal specs netiher MF imports..*)
 
 Ltac start_function_hint ::= idtac. (* no hint reminder *)
+
