VST-introduction/verif_client_pipe.v
@@ -1,9 +1,64 @@
 Require Import VST.floyd.proofauto.
+Require Import VC.ASI_kalloc.
 Require Import VC.client1.
 Require Import VC.helper.
+Require Import VC.VSU_kalloc_kfree_definitions.
+
 
 #[export] Instance CompSpecs : compspecs. make_compspecs prog. Defined.
-Definition Vprog : varspecs. mk_varspecs prog. Defined.
+(*Definition Vprog : varspecs. mk_varspecs prog. Defined.*)
+
+Definition MF_ASI: funspecs := Kalloc_ASI KF_APD _kalloc1 _kfree1.
+Definition MF_imported_specs:funspecs := nil.
+Definition MF_internal_specs: funspecs := MF_ASI.
+Definition MF_globals gv : mpred:= ASI_kalloc.mem_mgr KF_APD gv.
+Definition MFVprog : varspecs. mk_varspecs client1.prog. Defined.
+Definition MFGprog: funspecs := MF_imported_specs ++ MF_internal_specs.
 
 Local Open Scope logic.
 
+(*Require Import malloc.
+Require Import malloc_lemmas.
+Require Import malloc_sep.*)
+(*Require Import VC.VSU_kalloc_kfree_definitions.*)
+
+
+(*Definition Vprog : varspecs. mk_varspecs prog. Defined.*)
+
+
+
+Definition client_11_pipealloc_spec : ident * funspec :=
+ DECLARE _client_11_pipealloc
+ WITH (*sh : share, original_freelist_pointer:val, xx:Z, ls:list val,*) gv:globals
+ PRE [ ] 
+    PROP () PARAMS() GLOBALS(gv) SEP (MF_globals gv)
+ POST [ tvoid ] 
+    EX p: val, 
+    PROP ( ) RETURN () SEP (
+        if eq_dec p nullval then
+        emp
+        else 
+        kalloc_token' KF_APD Ews (sizeof t_struct_pipe) p *
+        pipe_rep Ews p * MF_globals gv).
+    
+
+Lemma body_pop: semax_body MFVprog MFGprog f_client_11_pipealloc client_11_pipealloc_spec.
+Proof.
+start_function.
+forward.
+forward_call (t_struct_pipe, gv). 
+- unfold MF_globals. entailer!.
+- Intros vret. forward_if.
+    + destruct (eq_dec vret nullval); entailer!. 
+    + destruct (eq_dec vret nullval).
+        * rewrite e in H. auto_contradict.
+        * rewrite mem_mgr_split. Intros sh ls xx original_freelist_pointer.
+        forward. forward. forward. forward. Exists vret.
+        destruct (eq_dec vret nullval); auto_contradict.
+        entailer.
+        unfold pipe_rep. entailer!.
+        unfold MF_globals. rewrite mem_mgr_split. Exists sh ls xx original_freelist_pointer. entailer!.
+        apply derives_refl.
+    + destruct (eq_dec vret nullval); auto_contradict.
+      forward. Exists vret. destruct (eq_dec vret nullval) eqn:e1; auto_contradict. entailer.
+Qed.
