VST-introduction/verif_kalloc1_kfree1.v
@@ -3,8 +3,8 @@ Require Import VC.ASI_kalloc.
 Require Import VC.client1.
 Require Import VC.helper.
 
-#[export] Instance CompSpecs : compspecs. make_compspecs prog. Defined.
-Definition Vprog : varspecs. mk_varspecs prog. Defined.
+(*#[export] Instance CompSpecs : compspecs. make_compspecs prog. Defined.
+Definition Vprog : varspecs. mk_varspecs prog. Defined.*)
 
 Local Open Scope logic.
 
@@ -15,8 +15,56 @@ Require Import VC.VSU_kalloc_kfree_definitions.
 
 Lemma body_kfree1 i: semax_body MF_Vprog MF_Gprog f_kfree1 (kfree1_spec KF_APD i).
 Proof. start_function.
+forward.
+rewrite mem_mgr_split.
+Intros sh ls xx original_freelist_pointer.
+destruct (eq_dec new_head nullval).
+- forward_if.
+    + rewrite e in H2; auto_contradict.
+    + forward. entailer.
+    rewrite mem_mgr_split. Exists sh ls xx original_freelist_pointer.
+    entailer!.
+- forward_if.
+    + Intros. forward. rewrite kalloc_token'_split. Intros v. forward. forward. entailer.
+    rewrite mem_mgr_split. Exists sh (original_freelist_pointer::ls) xx new_head. entailer!. 
+        * right; split; auto. unfold not; intros; auto_contradict.
+        * refold_freelistrep. entailer. admit.
+    + forward. entailer.
 Admitted.
 
-Lemma body_kalloc1 i: semax_body MF_Vprog MF_Gprog f_kalloc1 (kalloc1_spec KF_APD i).
-Proof. start_function. 
-Admitted.
+
+Lemma body_kalloc1 i: semax_body MF_Vprog MF_Gprog f_kalloc1 (kalloc1_spec (KF_APD) i).
+Proof. start_function.
+rewrite mem_mgr_split. Intros sh ls xx original_freelist_pointer.
+unfold abbreviate in POSTCONDITION.
+forward; forward_if (
+    PROP  ( )
+    LOCAL (
+        temp _r original_freelist_pointer; 
+        gvars gv
+        )
+    SEP (
+        ASI_kalloc.mem_mgr KF_APD gv;
+                   if eq_dec original_freelist_pointer nullval
+                   then emp
+                   else kalloc_token' KF_APD Ews PGSIZE original_freelist_pointer
+    )
+)%assert; 
+try (rewrite H012 in H; auto_contradict).
++ destruct H0 as [[H0011 H0012] | [H0021 H0022]].
+    - rewrite H0012 in H1; auto_contradict.
+    - destruct ls; auto_contradict.
+    refold_freelistrep. Intros.
+    forward. forward.
+    destruct (eq_dec original_freelist_pointer nullval) eqn:e1; auto_contradict. entailer.
+    rewrite mem_mgr_split. Exists sh (v::ls) xx original_freelist_pointer. entailer!.
+    refold_freelistrep. entailer.
+    rewrite kalloc_token'_split. Exists v. entailer. admit.
++ forward. destruct (eq_dec original_freelist_pointer nullval) eqn:e1; auto_contradict. entailer.
+    rewrite mem_mgr_split. Exists sh ([]:list val) xx nullval. entailer!. destruct H0 as [[H011 H012]| [H021 H022]]; auto_contradict.
+    rewrite H011. entailer.
++ destruct (eq_dec original_freelist_pointer nullval) eqn:e1. 
+    *forward. Exists nullval. entailer.
+    * forward. Exists original_freelist_pointer. entailer!. destruct (eq_dec original_freelist_pointer nullval) eqn:e2; auto_contradict.
+    entailer.
+Admitted. 
